Prove let soundness with method calls

JaIrisSoundness.v
@@ -1870,7 +1870,7 @@ Proof.
     rewrite StrMapFacts.add_eq_o.
     ++ apply (SuccessfullAllocIsNotNull CC h cn ls newloc newheap alloc_newloc_newheap).
     ++ trivial.
-Admitted.
+Qed.
 Hint Resolve HTNewNotNullRuleSoundness : core.
 
 Lemma HTNewFieldRuleSoundness : forall decls gamma cn objflds vs n field value s p mu v CC,
@@ -1933,6 +1933,25 @@ Lemma SubstExprEqExprSubstituteVal : forall x l e,
 Proof.
 Admitted.
 
+Lemma RedIsNoneIsFalseImpliesRedIsSome : forall CC conf p,
+  match red CC conf with
+  | Some (h, st) => p h st
+  | None => False
+  end -> exists h st, (red CC conf = Some (h, st) /\ p h st).
+Proof.
+  intros.
+  destruct (Classical_Prop.classic (exists h st, red CC conf = Some (h, st))).
+  + destruct H0 as (h & (st & red_is_some)).
+    exists h, st.
+    rewrite red_is_some in H.
+    exact (conj red_is_some H).
+  + destruct (red CC conf).
+    ++ destruct p0.
+       exists h, f.
+       split; try trivial.
+    ++ destruct H.
+Qed.
+
 Lemma EvaluationSplit : forall h st confs hn confs1 res h' st' CC,
   let stn := [ [] [[JFVal1 (JFVLoc res) ]]_ None] in
   (JFIPartialEval h st confs hn stn CC) ->
@@ -1951,19 +1970,38 @@ Proof.
     auto.
 Qed.
 
-Definition ExprRedPreservesContexts expr := forall h0 ctx class x e2 confs hn res CC,
-  (JFIPartialEval h0
-             [(ctx ++ [JFCtxLet class x __ e2]) [[ expr ]]_ None] confs hn
-             [ [] [[JFVal1 (JFVLoc res) ]]_ None] CC) ->
-  exists ctx' h' e1',
-    red CC (h0, [(ctx ++ [JFCtxLet class x __ e2]) [[ expr ]]_ None]) = 
-      Some (h', [(ctx' ++ ctx ++ [JFCtxLet class x __ e2]) [[ e1' ]]_ None]).
+Lemma SinglAppIsCons : forall A l (x : A), [x] ++ l = x::l.
+Proof.
+Admitted.
 
-Lemma NewEvalPreservesContexts : forall mu cn vs, ExprRedPreservesContexts (JFNew mu cn vs).
+Lemma app_split : forall T (a : T) l b,
+(a :: l) ++ [b] = [a] ++ l ++ [b].
+Proof.
+Admitted.
+
+Definition InnerExprRedPreservesLetCtx expr := forall h0 ctx class x e2 confs hn res CC,
+  (JFIPartialEval h0
+     [(ctx ++ [JFCtxLet class x __ e2]) [[ expr ]]_ None]
+      confs hn [ [] [[JFVal1 (JFVLoc res) ]]_ None] CC) ->
+  exists st' ctx' h' e1',
+    red CC (h0, [(ctx ++ [JFCtxLet class x __ e2]) [[ expr ]]_ None]) = 
+      Some (h', st' ++ [(ctx' ++ [JFCtxLet class x __ e2]) [[ e1' ]]_ None]).
+
+Definition OuterExprRedPreservesLetCtx expr := forall h0 st ctx let_ctx class x e1 e2 confs hn res A CC,
+  (JFIPartialEval h0
+     ([ctx [[ expr ]]_ A] ++ st ++ [(let_ctx ++ [JFCtxLet class x __ e2]) [[ e1 ]]_ None])
+      confs hn [ [] [[JFVal1 (JFVLoc res) ]]_ None] CC) ->
+  exists st' ctx' h' e1',
+    red CC (h0, [ctx [[ expr ]]_ A] ++ st ++ [(let_ctx ++ [JFCtxLet class x __ e2]) [[ e1 ]]_ None]) =
+      Some (h', st' ++ [(ctx' ++ [JFCtxLet class x __ e2]) [[ e1' ]]_ None]).
+
+
+Lemma NewInnerRedPreservesLetCtx : forall mu cn vs, InnerExprRedPreservesLetCtx (JFNew mu cn vs).
 Proof.
   intros mu cn vs h0 ctx class x e2 confs hn res CC.
   intros let_eval.
-  exists [].
+
+  exists [], ctx.
   unfold JFIPartialEval in let_eval;
   destruct confs; try discriminate (proj2 let_eval);
   fold JFIPartialEval in let_eval.
@@ -1989,11 +2027,39 @@ Proof.
     trivial.
 Qed.
 
-Lemma LetEvalPreservesContexts : forall cn x e1 e2, ExprRedPreservesContexts (JFLet cn x e1 e2).
+Lemma NewOuterRedPreservesLetCtx : forall mu cn vs, OuterExprRedPreservesLetCtx (JFNew mu cn vs).
+Proof.
+  intros mu cn vs h0 st ctx let_ctx class x e1 e2 confs hn res A CC.
+  intros let_eval.
+
+  unfold JFIPartialEval in let_eval;
+  destruct confs; try discriminate (proj2 let_eval);
+  fold JFIPartialEval in let_eval.
+  destruct p.
+  destruct let_eval as (_ & (_ & let_eval)).
+  unfold red in *.
+  rewrite SinglAppIsCons in *.
+
+  destruct ctx.
+  + destruct A; try destruct let_eval.
+    destruct (list_map_opt loc_of_val vs); try destruct let_eval.
+    destruct (alloc_init CC h0 cn l); try destruct let_eval.
+    destruct p.
+    exists (([] [[JFVal1 (JFVLoc l0) ]]_ None)::st), let_ctx, h1, e1.
+    trivial.
+  + destruct A; try (destruct j; destruct let_eval).
+    destruct (list_map_opt loc_of_val vs); try (destruct j; destruct let_eval).
+    destruct (alloc_init CC h0 cn l); try (destruct j; destruct let_eval).
+    destruct p.
+    exists (ctx _[ j _[[_ JFVal1 (JFVLoc l0) _]]_ None ]_ :: st), let_ctx, h1, e1.
+    destruct j; trivial.
+Qed.
+
+Lemma LetInnerRedPreservesLetCtx : forall cn x e1 e2, InnerExprRedPreservesLetCtx (JFLet cn x e1 e2).
 Proof.
   intros cn x e1 e2 h0 ctx outer_class outer_x outer_e2 confs hn res CC.
   intros let_eval.
-  exists ([JFCtxLet cn x __ e2]).
+  exists [], ([JFCtxLet cn x __ e2] ++ ctx).
 
   unfold JFIPartialEval in let_eval;
   destruct confs; try discriminate (proj2 let_eval);
@@ -2002,43 +2068,681 @@ Proof.
   destruct let_eval as (_ & (_ & let_eval)).
   unfold red in *.
 
-  assert (ctx_has_head := concatNonemptyHasHead JFContextNode ctx (JFCtxLet outer_class outer_x __ outer_e2)).
-  destruct ctx_has_head as (ctx_h & (ctx_l & ctx_concat)).
+  destruct (concatNonemptyHasHead JFContextNode ctx (JFCtxLet outer_class outer_x __ outer_e2))
+   as (ctx_h & (ctx_l & ctx_concat)).
   rewrite ctx_concat.
   rewrite <- ctx_concat.
   exists h0, e1.
   destruct ctx_h; trivial.
 Qed.
 
-Lemma IfEvalPreservesContexts : forall v1 v2 e1 e2, ExprRedPreservesContexts (JFIf v1 v2 e1 e2).
+Lemma LetOuterRedPreservesLetCtx : forall cn x e1 e2, OuterExprRedPreservesLetCtx (JFLet cn x e1 e2).
 Proof.
+  intros cn x e1 e2 h0 st ctx let_ctx outer_class outer_x outer_e1 outer_e2 confs hn res A CC.
+  intros let_eval.
+
+  unfold JFIPartialEval in let_eval;
+  destruct confs; try discriminate (proj2 let_eval);
+  fold JFIPartialEval in let_eval.
+  destruct p.
+  destruct let_eval as (_ & (_ & let_eval)).
+  unfold red in *.
+  rewrite SinglAppIsCons in *.
+
+  destruct ctx.
+  + exists ([ [] _[ JFCtxLet cn x __ e2 _[[_ e1 _]]_ None ]_ ] ++ st), let_ctx, h0, outer_e1.
+    destruct A; try destruct let_eval; try trivial.
+  + destruct j; destruct A; try destruct let_eval.
+    ++ exists ((JFCtxLet C x0 Ctx E2 :: ctx) _[ JFCtxLet cn x __ e2 _[[_ e1 _]]_ None ]_ :: st),
+          let_ctx, h0, outer_e1.
+       trivial.
+    ++ exists ((JFCtxTry Ctx mu C x0 E2 :: ctx) _[ JFCtxLet cn x __ e2 _[[_ e1 _]]_ None ]_ :: st),
+          let_ctx, h0, outer_e1.
+       trivial.
+Qed.
+
+Lemma IfInnerRedPreservesLetCtx : forall v1 v2 e1 e2, InnerExprRedPreservesLetCtx (JFIf v1 v2 e1 e2).
+Proof.
+  intros v1 v2 e1 e2 h0 ctx outer_class outer_x outer_e2 confs hn res CC.
+  intros let_eval.
+  exists [], ctx, h0.
+
+  unfold JFIPartialEval in let_eval;
+  destruct confs; try discriminate (proj2 let_eval);
+  fold JFIPartialEval in let_eval.
+  destruct p.
+  destruct let_eval as (_ & (_ & let_eval)).
+  unfold red in *.
+  destruct (concatNonemptyHasHead JFContextNode ctx (JFCtxLet outer_class outer_x __ outer_e2))
+   as (ctx_h & (ctx_l & ctx_concat)).
+  rewrite ctx_concat in *.
+
+  destruct v1, v2; try (destruct ctx_h; destruct let_eval).
+
+  destruct (Loc_dec l l0).
+  + exists e1.
+    destruct ctx_h; trivial.
+  + exists e2.
+    destruct ctx_h; trivial.
+Qed.
+
+Lemma IfOuterRedPreservesLetCtx : forall v1 v2 e1 e2, OuterExprRedPreservesLetCtx (JFIf v1 v2 e1 e2).
+Proof.
+  intros v1 v2 e1 e2 h0 st ctx let_ctx outer_class outer_x outer_e1 outer_e2 confs hn res A CC.
+  intros let_eval.
+
+  unfold JFIPartialEval in let_eval;
+  destruct confs; try discriminate (proj2 let_eval);
+  fold JFIPartialEval in let_eval.
+  destruct p.
+  destruct let_eval as (_ & (_ & let_eval)).
+  unfold red in *.
+  rewrite SinglAppIsCons in *.
+
+  destruct v1, v2; try (destruct ctx as [ | j]; try destruct j; destruct let_eval).
+  destruct A.
+  + destruct ctx as [ | j0]; try destruct j0; try destruct let_eval.
+  + destruct (Loc_dec l l0).
+    ++ exists ((ctx [[ e1 ]]_ None)::st), let_ctx, h0, outer_e1.
+       destruct ctx; trivial.
+       destruct j; trivial.
+    ++ exists ((ctx [[ e2 ]]_ None)::st), let_ctx, h0, outer_e1.
+       destruct ctx; trivial.
+       destruct j; trivial.
+Qed.
+
+Lemma InvokeInnerRedPreservesLetCtx : forall v m vs, InnerExprRedPreservesLetCtx (JFInvoke v m vs).
+Proof.
+  intros v m vs h0 ctx outer_class outer_x outer_e2 confs hn res CC.
+  intros let_eval.
+
+  unfold JFIPartialEval in let_eval;
+  destruct confs; try discriminate (proj2 let_eval);
+  fold JFIPartialEval in let_eval.
+  destruct p.
+  destruct let_eval as (_ & (_ & let_eval)).
+  unfold red in *.
+  destruct (concatNonemptyHasHead JFContextNode ctx (JFCtxLet outer_class outer_x __ outer_e2))
+   as (ctx_h & (ctx_l & ctx_concat)).
+  rewrite ctx_concat in *.
+
+  destruct v; try (destruct ctx_h; destruct let_eval).
+  destruct l.
+  + admit. (* TODO exception *)
+  + destruct ctx_h.
+    ++ unfold getInvokeBody in *.
+       destruct getClassName; try destruct let_eval.
+       destruct methodLookup; try destruct let_eval.
+       destruct substList; try destruct let_eval.
+       rewrite <- ctx_concat.
+       exists ([ [] [[j1 ]]_ None ]), ctx, h0, (JFInvoke (JFVLoc (JFLoc n)) m vs).
+       trivial.
+    ++ unfold getInvokeBody in *.
+       destruct getClassName; try destruct let_eval.
+       destruct methodLookup; try destruct let_eval.
+       destruct substList; try destruct let_eval.
+       rewrite <- ctx_concat.
+       exists ([ [] [[j1 ]]_ None ]), ctx, h0, (JFInvoke (JFVLoc (JFLoc n)) m vs).
+       trivial.
 Admitted.
 
-(* ... *)
+Lemma InvokeOuterRedPreservesLetCtx : forall v m vs, OuterExprRedPreservesLetCtx (JFInvoke v m vs).
+Proof.
+  intros v m vs h0 st ctx let_ctx class x e1 e2 confs hn res A CC.
+  intros let_eval.
 
-(* TODO przy invoke moze dojsc nowa ramka na stos *)
-Lemma LetCtxIsValOrRedToLetCtx : forall h0 class x e1 e2 confs hn res CC ctx,
+  unfold JFIPartialEval in let_eval;
+  destruct confs; try discriminate (proj2 let_eval);
+  fold JFIPartialEval in let_eval.
+  destruct p.
+  destruct let_eval as (_ & (_ & let_eval)).
+  unfold red in *.
+  rewrite SinglAppIsCons in *.
+
+  destruct A; try (
+   destruct ctx; destruct v as [ | l];
+   destruct l; try destruct j0; destruct let_eval).
+
+  destruct ctx, v; try destruct let_eval.
+  + destruct l.
+    ++ exists (([] [[JFVal1 NPE_val ]]_ NPE_mode)::st), let_ctx, h0, e1.
+       trivial.
+    ++ unfold getInvokeBody in *.
+       destruct getClassName; try destruct let_eval.
+       destruct methodLookup; try destruct let_eval.
+       destruct substList; try destruct let_eval.
+       exists (([] [[j1 ]]_ None)::([] [[JFInvoke (JFVLoc (JFLoc n)) m vs ]]_ None)::st),
+          let_ctx, h0, e1.
+       trivial.
+  + destruct j.
+    ++ destruct l.
+       +++ exists (ctx _[ JFCtxLet C x0 Ctx E2 _[[_ JFVal1 NPE_val _]]_ NPE_mode ]_::st),
+              let_ctx, h0, e1.
+           trivial.
+       +++ unfold getInvokeBody in *.
+           destruct getClassName; try destruct let_eval.
+           destruct methodLookup; try destruct let_eval.
+           destruct substList; try destruct let_eval.
+            exists (([] [[j1 ]]_ None)
+              ::ctx _[ JFCtxLet C x0 Ctx E2 _[[_ JFInvoke (JFVLoc (JFLoc n)) m vs _]]_ None ]_ 
+              ::st),
+              let_ctx, h0, e1.
+           trivial.
+    ++ destruct l.
+       +++ exists (ctx _[ JFCtxTry Ctx mu C x0 E2 _[[_ JFVal1 NPE_val _]]_ NPE_mode ]_ :: st),
+              let_ctx, h0, e1.
+           trivial.
+       +++ unfold getInvokeBody in *.
+           destruct getClassName; try destruct let_eval.
+           destruct methodLookup; try destruct let_eval.
+           destruct substList; try destruct let_eval.
+            exists (([] [[j1 ]]_ None)
+              ::ctx _[ JFCtxTry Ctx mu C x0 E2 _[[_ JFInvoke (JFVLoc (JFLoc n)) m vs _]]_ None ]_ 
+              ::st),
+              let_ctx, h0, e1.
+           trivial.
+  + destruct j; destruct let_eval.
+Qed.
+
+Lemma AssignInnerRedPreservesLetCtx : forall vx v, InnerExprRedPreservesLetCtx (JFAssign vx v).
+Proof.
+  intros vx v h0 ctx outer_class outer_x outer_e2 confs hn res CC.
+  intros let_eval.
+
+  unfold JFIPartialEval in let_eval;
+  destruct confs; try discriminate (proj2 let_eval);
+  fold JFIPartialEval in let_eval.
+  destruct p.
+  destruct let_eval as (_ & (_ & let_eval)).
+  destruct (concatNonemptyHasHead JFContextNode ctx (JFCtxLet outer_class outer_x __ outer_e2))
+   as (ctx_h & (ctx_l & ctx_concat)).
+  rewrite ctx_concat in *.
+
+  unfold red in *.
+  destruct vx.
+  destruct v; try (
+    destruct ctx_h; destruct j as [ | l];
+    try destruct l; destruct let_eval
+  ).
+  destruct j.
+  + destruct ctx_h.
+    ++ destruct l0; try destruct let_eval.
+       +++ admit. (* TODO exception *)
+       +++ destruct (Heap.find (elt:=Obj) n h0); try destruct let_eval.
+           destruct o.
+           rewrite <- ctx_concat.
+           exists [], ctx, (Heap.add n (JFXIdMap.add j0 l r, j) h0), (JFVal1 (JFVLoc l)).
+           trivial.
+    ++ destruct l0; try destruct let_eval.
+       +++ admit. (* TODO exception *)
+       +++ destruct (Heap.find (elt:=Obj) n h0); try destruct let_eval.
+           destruct o.
+           rewrite <- ctx_concat.
+           exists [], ctx, (Heap.add n (JFXIdMap.add j0 l r, j) h0), (JFVal1 (JFVLoc l)).
+           trivial.
+  + admit. (* TODO exception *)
+Admitted.
+
+Lemma AssignOuterRedPreservesLetCtx : forall vx v, OuterExprRedPreservesLetCtx (JFAssign vx v).
+Proof.
+  intros vx v h0 st ctx let_ctx class x e1 e2 confs hn res A CC.
+  intros let_eval.
+
+  unfold JFIPartialEval in let_eval;
+  destruct confs; try discriminate (proj2 let_eval);
+  fold JFIPartialEval in let_eval.
+  destruct p.
+  destruct let_eval as (_ & (_ & let_eval)).
+  rewrite SinglAppIsCons in *.
+  unfold red in *.
+
+  destruct vx.
+  destruct ctx.
+  + destruct j; try destruct let_eval.
+    destruct l.
+    ++ destruct A, v; try destruct let_eval.
+       exists (([] [[JFVal1 NPE_val ]]_ NPE_mode)::st), let_ctx, h0, e1.
+       trivial.
+    ++ destruct A, v; try destruct let_eval.
+       destruct (Heap.find (elt:=Obj) n h0); try destruct let_eval.
+       destruct o.
+       exists (([] [[JFVal1 (JFVLoc l) ]]_ None)::st), let_ctx, (Heap.add n (JFXIdMap.add j0 l r, j) h0), e1.
+       trivial.
+  + destruct j; try destruct let_eval.
+    ++ destruct l.
+       +++ destruct A, v; try (destruct j1; destruct let_eval).
+           destruct j1.
+           - exists (ctx _[ JFCtxLet C x0 Ctx E2 _[[_ JFVal1 NPE_val _]]_ NPE_mode ]_::st), let_ctx, h0, e1.
+             trivial.
+           - exists (ctx _[ JFCtxTry Ctx mu C x0 E2 _[[_ JFVal1 NPE_val _]]_ NPE_mode ]_::st), let_ctx, h0, e1.
+             trivial.
+       +++ destruct A, v; try (destruct j1; destruct let_eval).
+           destruct j1.
+           - destruct (Heap.find (elt:=Obj) n h0); try destruct let_eval.
+             destruct o.
+             exists (ctx _[ JFCtxLet C x0 Ctx E2 _[[_ JFVal1 (JFVLoc l) _]]_ None ]_::st), let_ctx,
+                (Heap.add n (JFXIdMap.add j0 l r, j) h0), e1.
+             trivial.
+           - destruct (Heap.find (elt:=Obj) n h0); try destruct let_eval.
+             destruct o.
+             exists (ctx _[ JFCtxTry Ctx mu C x0 E2 _[[_ JFVal1 (JFVLoc l) _]]_ None ]_::st), let_ctx,
+                (Heap.add n (JFXIdMap.add j0 l r, j) h0), e1.
+             trivial.
+    ++ destruct j1; try destruct let_eval.
+Qed.
+
+Lemma Val1InnerRedPreservesLetCtx : forall v h0 ctx ctxs outer_class outer_x outer_e2 confs hn res CC,
+  (JFIPartialEval h0 [((ctx::ctxs) ++ [JFCtxLet outer_class outer_x __ outer_e2]) [[ JFVal1 v ]]_ None] confs 
+                  hn [ [] [[JFVal1 (JFVLoc res) ]]_ None] CC) ->
+  exists st' ctx' h' e1',
+    red CC (h0, [((ctx::ctxs) ++ [JFCtxLet outer_class outer_x __ outer_e2]) [[ JFVal1 v ]]_ None]) = 
+      Some (h', st' ++ [(ctx' ++ [JFCtxLet outer_class outer_x __ outer_e2]) [[ e1' ]]_ None]).
+Proof.
+  intros v h0 ctx ctxs outer_class outer_x outer_e2 confs hn res CC.
+  intros let_eval.
+
+  unfold JFIPartialEval in let_eval;
+  destruct confs; try discriminate (proj2 let_eval);
+  fold JFIPartialEval in let_eval.
+  destruct p.
+  destruct let_eval as (_ & (_ & let_eval)).
+
+  unfold red in *.
+  rewrite <- app_comm_cons in *.
+  destruct v; try (destruct ctx; destruct let_eval).
+  destruct ctx.
+  + exists [], ctxs, h0, (substExpr (JFVar x) l E2).
+    trivial.
+  + exists [], ctxs, h0, (JFVal1 (JFVLoc l)).
+    trivial.
+Qed.
+
+Lemma Val1OuterRedPreservesLetCtx : forall v, OuterExprRedPreservesLetCtx (JFVal1 v).
+Proof.
+  intros v h0 st ctx let_ctx class x e1 e2 confs hn res A CC.
+  intros let_eval.
+
+  unfold JFIPartialEval in let_eval.
+  destruct confs.
+  + destruct let_eval as (h_eq & let_eval).
+    apply app_eq_unit in let_eval.
+    destruct let_eval.
+    ++ discriminate (proj1 H).
+    ++ destruct H as (_ & H).
+       apply app_eq_nil in H.
+       discriminate (proj2 H).
+  + destruct p.
+    fold JFIPartialEval in let_eval.
+    destruct let_eval as (h_eq & (ctx_eq & let_eval)).
+    rewrite SinglAppIsCons in *.
+    unfold red in *.
+   destruct v; try (destruct ctx as [ | j]; try destruct j; destruct let_eval).
+   destruct ctx.
+   ++ destruct A.
+      +++ destruct st.
+          - rewrite app_nil_l in *.
+            destruct e1; try destruct let_eval.
+            admit. (* TODO exception *)
+          - rewrite <- app_comm_cons in *.
+          destruct f0; try destruct let_eval.
+          destruct E; try destruct let_eval.
+          destruct A; try destruct let_eval.
+          exists ((Ctx [[JFVal1 (JFVLoc l) ]]_ Some j)::st), let_ctx, h0, e1.
+          trivial.
+      +++ destruct st.
+          - rewrite app_nil_l in *.
+            destruct e1; try destruct let_eval.
+            exists [], let_ctx, h0, (JFVal1 (JFVLoc l)).
+            trivial.
+          - rewrite <- app_comm_cons in *.
+          destruct f0; try destruct let_eval.
+          destruct E; try destruct let_eval.
+          destruct A; try destruct let_eval.
+          exists ((Ctx [[JFVal1 (JFVLoc l) ]]_ None)::st), let_ctx, h0, e1.
+          trivial.
+   ++ destruct A.
+      +++ destruct st.
+          - rewrite app_nil_l in *.
+            destruct j.
+            -- exists [ctx [[JFVal1 (JFVLoc l) ]]_ Some j0], let_ctx, h0, e1.
+               trivial.
+            -- destruct (JaSubtype.subtype_bool CC (JFClass j0) (JFClass C)).
+               --- exists [ctx [[substExpr (JFVar x0) l E2 ]]_ None], let_ctx, h0, e1.
+                   trivial.
+               --- exists [ctx [[JFVal1 (JFVLoc l) ]]_ Some j0], let_ctx, h0, e1.
+                   trivial.
+          - destruct j.
+            -- exists ((ctx [[JFVal1 (JFVLoc l) ]]_ Some j0)::(f0 :: st)), let_ctx, h0, e1.
+               trivial.
+            -- destruct (JaSubtype.subtype_bool CC (JFClass j0) (JFClass C)).
+               --- exists ((ctx [[substExpr (JFVar x0) l E2 ]]_ None)::(f0 :: st)), let_ctx, h0, e1.
+                   trivial.
+               --- exists ((ctx [[JFVal1 (JFVLoc l) ]]_ Some j0)::(f0 :: st)), let_ctx, h0, e1.
+                   trivial.
+      +++ destruct st.
+          - destruct j.
+            -- exists [ctx [[substExpr (JFVar x0) l E2 ]]_ None], let_ctx, h0, e1.
+               trivial.
+            -- exists [ctx [[JFVal1 (JFVLoc l) ]]_ None], let_ctx, h0, e1.
+               trivial.
+          - destruct j.
+            -- exists ((ctx [[substExpr (JFVar x0) l E2 ]]_ None)::(f0::st)), let_ctx, h0, e1.
+               trivial.
+            -- exists ((ctx [[JFVal1 (JFVLoc l) ]]_ None)::(f0::st)), let_ctx, h0, e1.
+               trivial.
+Admitted.
+
+Lemma Val2InnerRedPreservesLetCtx : forall vx, InnerExprRedPreservesLetCtx (JFVal2 vx).
+Proof.
+  intros vx h0 ctx outer_class outer_x outer_e2 confs hn res CC.
+  intros let_eval.
+
+  unfold JFIPartialEval in let_eval;
+  destruct confs; try discriminate (proj2 let_eval);
+  fold JFIPartialEval in let_eval.
+  destruct p.
+  destruct let_eval as (_ & (_ & let_eval)).
+  destruct (concatNonemptyHasHead JFContextNode ctx (JFCtxLet outer_class outer_x __ outer_e2))
+   as (ctx_h & (ctx_l & ctx_concat)).
+  rewrite ctx_concat in *.
+
+  unfold red in *.
+  destruct vx.
+  destruct j as [ | l]; try (destruct l; destruct ctx_h; destruct let_eval).
+  destruct ctx_h.
+  + destruct l.
+    ++ admit. (* TODO exception *)
+    ++ destruct (Heap.find (elt:=Obj) n h0); try destruct let_eval.
+       destruct o.
+       destruct (JFXIdMap.find (elt:=Loc) j0 r); try destruct let_eval.
+       rewrite <- ctx_concat.
+       exists [], ctx, h0, (JFVal1 (JFVLoc l)).
+       trivial.
+  + destruct l.
+    ++ admit. (* TODO exception *)
+    ++ destruct (Heap.find (elt:=Obj) n h0); try destruct let_eval.
+       destruct o.
+       destruct (JFXIdMap.find (elt:=Loc) j0 r); try destruct let_eval.
+       rewrite <- ctx_concat.
+       exists [], ctx, h0, (JFVal1 (JFVLoc l)).
+       trivial.
+Admitted.
+
+Lemma Val2OuterRedPreservesLetCtx : forall vx, OuterExprRedPreservesLetCtx (JFVal2 vx).
+Proof.
+  intros vx h0 st ctx let_ctx class x e1 e2 confs hn res A CC.
+  intros let_eval.
+
+  unfold JFIPartialEval in let_eval;
+  destruct confs; try discriminate (proj2 let_eval);
+  fold JFIPartialEval in let_eval.
+  destruct p.
+  destruct let_eval as (_ & (_ & let_eval)).
+  rewrite SinglAppIsCons in *.
+  unfold red in *.
+
+  destruct vx.
+  destruct A; try (
+    destruct ctx as [ | j2]; try destruct j2;
+    destruct j as [ | l]; try destruct l; destruct let_eval).
+  destruct ctx.
+  + destruct j; try destruct let_eval.
+    destruct l; try destruct let_eval.
+    ++ exists (([] [[JFVal1 NPE_val ]]_ NPE_mode)::st), let_ctx, h0, e1.
+       trivial.
+    ++ destruct (Heap.find (elt:=Obj) n h0); try destruct let_eval.
+       destruct o.
+       destruct (JFXIdMap.find (elt:=Loc) j0 r); try destruct let_eval.
+       exists (([] [[JFVal1 (JFVLoc l) ]]_ None)::st), let_ctx, h0, e1.
+       trivial.
+  + destruct j.
+    ++ destruct j1.
+       +++ destruct l; try destruct let_eval.
+           - exists ((ctx _[ JFCtxLet C x0 Ctx E2 _[[_ JFVal1 NPE_val _]]_ NPE_mode ]_)::st), let_ctx, h0, e1.
+             trivial.
+           - destruct (Heap.find (elt:=Obj) n h0); try destruct let_eval.
+             destruct o.
+             destruct (JFXIdMap.find (elt:=Loc) j0 r); try destruct let_eval.
+             exists ((ctx _[ JFCtxLet C x0 Ctx E2 _[[_ JFVal1 (JFVLoc l) _]]_ None ]_)::st), let_ctx, h0, e1.
+             trivial.
+       +++ destruct l; try destruct let_eval.
+           - exists ((ctx _[ JFCtxTry Ctx mu C x0 E2 _[[_ JFVal1 NPE_val _]]_ NPE_mode ]_)::st), let_ctx, h0, e1.
+             trivial.
+           - destruct (Heap.find (elt:=Obj) n h0); try destruct let_eval.
+             destruct o.
+             destruct (JFXIdMap.find (elt:=Loc) j0 r); try destruct let_eval.
+             exists ((ctx _[ JFCtxTry Ctx mu C x0 E2 _[[_ JFVal1 (JFVLoc l) _]]_ None ]_)::st), let_ctx, h0, e1.
+             trivial.
+    ++ destruct j1; try destruct let_eval.
+Qed.
+
+Lemma ThrowInnerRedPreservesLetCtx : forall v, InnerExprRedPreservesLetCtx (JFThrow v).
+Proof.
+  intros v h0 ctx outer_class outer_x outer_e2 confs hn res CC.
+  intros let_eval.
+
+  unfold JFIPartialEval in let_eval;
+  destruct confs; try discriminate (proj2 let_eval);
+  fold JFIPartialEval in let_eval.
+  destruct p.
+  destruct let_eval as (_ & (_ & let_eval)).
+  destruct (concatNonemptyHasHead JFContextNode ctx (JFCtxLet outer_class outer_x __ outer_e2))
+   as (ctx_h & (ctx_l & ctx_concat)).
+  rewrite ctx_concat in *.
+
+  unfold red in *.
+  destruct v; try (destruct ctx_h; destruct let_eval).
+  destruct ctx_h.
+  + destruct l.
+    ++ admit. (* TODO exception *)
+    ++ destruct (class h0 n); try destruct let_eval.
+       rewrite <- ctx_concat.
+       admit. (* TODO exception *)
+  + destruct l.
+    ++ admit. (* TODO exception *)
+    ++ destruct (class h0 n); try destruct let_eval.
+       rewrite <- ctx_concat.
+       admit. (* TODO exception *)
+Admitted.
+
+Lemma ThrowOuterRedPreservesLetCtx : forall v, OuterExprRedPreservesLetCtx (JFThrow v).
+Proof.
+  intros v h0 st ctx let_ctx class x e1 e2 confs hn res A CC.
+  intros let_eval.
+
+  unfold JFIPartialEval in let_eval;
+  destruct confs; try discriminate (proj2 let_eval);
+  fold JFIPartialEval in let_eval.
+  destruct p.
+  destruct let_eval as (_ & (_ & let_eval)).
+  rewrite SinglAppIsCons in *.
+  unfold red in *.
+  destruct A; try (
+    destruct ctx as [ | j0]; try destruct j0;
+    destruct v as [ | l]; try destruct l; destruct let_eval).
+  destruct ctx.
+  + destruct v; try destruct let_eval.
+    destruct l.
+    ++ exists (([] [[JFVal1 NPE_val ]]_ NPE_mode)::st), let_ctx, h0, e1.
+       trivial.
+    ++ destruct (Jafun.class h0 n); try destruct let_eval.
+       exists (([] [[JFVal1 (JFVLoc (JFLoc n)) ]]_ Some j)::st), let_ctx, h0, e1.
+       trivial.
+  + destruct j.
+    ++ destruct v; try destruct let_eval.
+       destruct l.
+       +++ exists (( ctx _[ JFCtxLet C x0 Ctx E2 _[[_ JFVal1 NPE_val _]]_ NPE_mode ]_)::st), let_ctx, h0, e1.
+           trivial.
+       +++ destruct (Jafun.class h0 n); try destruct let_eval.
+           exists ((ctx _[ JFCtxLet C x0 Ctx E2 _[[_ JFVal1 (JFVLoc (JFLoc n)) _]]_ Some j ]_)::st), let_ctx, h0, e1.
+           trivial.
+    ++ destruct v; try destruct let_eval.
+       destruct l.
+       +++ exists (( ctx _[ JFCtxTry Ctx mu C x0 E2 _[[_ JFVal1 NPE_val _]]_ NPE_mode ]_)::st), let_ctx, h0, e1.
+           trivial.
+       +++ destruct (Jafun.class h0 n); try destruct let_eval.
+           exists ((ctx _[ JFCtxTry Ctx mu C x0 E2 _[[_ JFVal1 (JFVLoc (JFLoc n)) _]]_ Some j ]_)::st), let_ctx, h0, e1.
+           trivial.
+Qed.
+
+Lemma TryInnerRedPreservesLetCtx : forall e1 mu cn x0 e2, InnerExprRedPreservesLetCtx (JFTry e1 mu cn x0 e2).
+Proof.
+  intros e1 mu cn x0 e2 h0 ctx outer_class outer_x outer_e2 confs hn res CC.
+  intros let_eval.
+
+  unfold JFIPartialEval in let_eval;
+  destruct confs; try discriminate (proj2 let_eval);
+  fold JFIPartialEval in let_eval.
+  destruct p.
+  destruct let_eval as (_ & (_ & let_eval)).
+  destruct (concatNonemptyHasHead JFContextNode ctx (JFCtxLet outer_class outer_x __ outer_e2))
+   as (ctx_h & (ctx_l & ctx_concat)).
+  rewrite ctx_concat in *.
+  unfold red in *.
+  rewrite <- ctx_concat in *.
+  destruct ctx_h.
+  + exists [], ((JFCtxTry __ mu cn x0 e2)::ctx), h0, e1.
+    trivial.
+  + exists [], ((JFCtxTry __ mu cn x0 e2)::ctx), h0, e1.
+    trivial.
+Qed.
+
+Lemma TryOuterRedPreservesLetCtx : forall e1 mu cn x0 e2, OuterExprRedPreservesLetCtx (JFTry e1 mu cn x0 e2).
+Proof.
+  intros e1 mu cn x0 e2 h0 st ctx let_ctx outer_class outer_x outer_e1 outer_e2 confs hn res A CC.
+  intros let_eval.
+
+  unfold JFIPartialEval in let_eval;
+  destruct confs; try discriminate (proj2 let_eval);
+  fold JFIPartialEval in let_eval.
+  destruct p.
+  destruct let_eval as (_ & (_ & let_eval)).
+  rewrite SinglAppIsCons in *.
+  unfold red in *.
+  destruct ctx.
+  + destruct A; try destruct let_eval.
+    exists (([] _[ JFCtxTry __ mu cn x0 e2 _[[_ e1 _]]_ None ]_)::st), let_ctx, h0, outer_e1.
+    trivial.
+  + destruct A; try destruct let_eval.
+    destruct j; try destruct let_eval.
+    destruct j.
+    ++ exists (((JFCtxLet C x Ctx E2 :: ctx) _[ JFCtxTry __ mu cn x0 e2 _[[_ e1 _]]_ None ]_)::st), let_ctx, h0, outer_e1.
+       trivial.
+    ++ exists (((JFCtxTry Ctx mu0 C x E2:: ctx) _[ JFCtxTry __ mu cn x0 e2 _[[_ e1 _]]_ None ]_)::st), let_ctx, h0, outer_e1.
+       trivial.
+Qed.
+
+Lemma OnlyFrameIsValOrRedPreservesLetCtx : forall h0 class x e1 e2 confs hn res CC ctx,
   let st0 := [ (ctx ++ [JFCtxLet class x __ e2]) [[ e1 ]]_ None ] in
   JFIPartialEval h0 st0 confs hn [ [] [[JFVal1 (JFVLoc res) ]]_ None] CC ->
    (ctx = [] /\ exists e1_res, e1 = JFVal1 (JFVLoc e1_res)) \/
-   (exists ctx' h' e1', red CC (h0, st0) = Some (h', [ (ctx' ++ ctx ++ [JFCtxLet class x __ e2]) [[ e1' ]]_ None ])).
+   (exists st' ctx' h' e1', red CC (h0, st0) = Some (h', st' ++ [ (ctx' ++ [JFCtxLet class x __ e2]) [[ e1' ]]_ None ])).
 Proof.
-  intros h0 class x e1 e2 confs hn res CC.
+  intros h0 class x e1 e2 confs hn res CC ctx.
   destruct e1;
-    intros ctx st0 let_eval.
+    intros st0 let_eval.
   + apply or_intror.
-    unfold st0 in *.
-    apply NewEvalPreservesContexts with (confs := confs) (hn := hn) (res := res).
+    apply NewInnerRedPreservesLetCtx with (confs := confs) (hn := hn) (res := res).
     exact let_eval.
   + apply or_intror.
-    unfold st0 in *.
-    apply LetEvalPreservesContexts with (confs := confs) (hn := hn) (res := res).
+    apply LetInnerRedPreservesLetCtx with (confs := confs) (hn := hn) (res := res).
     exact let_eval.
   + apply or_intror.
-    unfold st0 in *.
-    apply IfEvalPreservesContexts with (confs := confs) (hn := hn) (res := res).
+    apply IfInnerRedPreservesLetCtx with (confs := confs) (hn := hn) (res := res).
     exact let_eval.
-Admitted.
+  + apply or_intror.
+    apply InvokeInnerRedPreservesLetCtx with (confs := confs) (hn := hn) (res := res).
+    exact let_eval.
+  + apply or_intror.
+    apply AssignInnerRedPreservesLetCtx with (confs := confs) (hn := hn) (res := res).
+    exact let_eval.
+  + destruct ctx.
+    ++ apply or_introl.
+       split; trivial.
+       destruct (EnsureValIsLoc v) as (e1_res & v_eq_e1_res).
+       exists e1_res.
+       rewrite v_eq_e1_res.
+       trivial.
+    ++ apply or_intror.
+       apply Val1InnerRedPreservesLetCtx with (confs := confs) (hn := hn) (res := res).
+       exact let_eval.
+  + apply or_intror.
+    apply Val2InnerRedPreservesLetCtx with (confs := confs) (hn := hn) (res := res).
+    exact let_eval.
+  + apply or_intror.
+    apply ThrowInnerRedPreservesLetCtx with (confs := confs) (hn := hn) (res := res).
+    exact let_eval.
+  + apply or_intror.
+    apply TryInnerRedPreservesLetCtx with (confs := confs) (hn := hn) (res := res).
+    exact let_eval.
+Qed.
+
+Lemma TopFrameRedPreservesLetCtx : forall h0 f st let_ctx class x e2 e1 confs hn res CC,
+  let st0 := [ f ] ++ st ++
+             [ (let_ctx ++ [JFCtxLet class x __ e2]) [[ e1 ]]_ None ] in
+  JFIPartialEval h0 st0 confs hn [ [] [[JFVal1 (JFVLoc res) ]]_ None] CC ->
+   (exists st' ctx' h' e1', red CC (h0, st0) = Some (h', st' ++ [ (ctx' ++ [JFCtxLet class x __ e2]) [[ e1' ]]_ None ])).
+Proof.
+  intros h0 f st let_ctx class x e2 e1 confs hn res CC.
+  intros st0 let_eval.
+  destruct f.
+  destruct E.
+  + unfold st0 in *.
+    apply NewOuterRedPreservesLetCtx with (confs := confs) (hn := hn) (res := res).
+    exact let_eval.
+  + unfold st0 in *.
+    apply LetOuterRedPreservesLetCtx with (confs := confs) (hn := hn) (res := res).
+    exact let_eval.
+  + unfold st0 in *.
+    apply IfOuterRedPreservesLetCtx with (confs := confs) (hn := hn) (res := res).
+    exact let_eval.
+  + unfold st0 in *.
+    apply InvokeOuterRedPreservesLetCtx with (confs := confs) (hn := hn) (res := res).
+    exact let_eval.
+  + unfold st0 in *.
+    apply AssignOuterRedPreservesLetCtx with (confs := confs) (hn := hn) (res := res).
+    exact let_eval.
+  + unfold st0 in *.
+    apply Val1OuterRedPreservesLetCtx with (confs := confs) (hn := hn) (res := res).
+    exact let_eval.
+  + unfold st0 in *.
+    apply Val2OuterRedPreservesLetCtx with (confs := confs) (hn := hn) (res := res).
+    exact let_eval.
+  + unfold st0 in *.
+    apply ThrowOuterRedPreservesLetCtx with (confs := confs) (hn := hn) (res := res).
+    exact let_eval.
+  + unfold st0 in *.
+    apply TryOuterRedPreservesLetCtx with (confs := confs) (hn := hn) (res := res).
+    exact let_eval.
+Qed.
+
+Lemma RedPreservesLetCtxUntilE2Evaluates : forall h0 class x e1 e2 confs hn res CC st ctx,
+  let st0 := st ++ [ (ctx ++ [JFCtxLet class x __ e2]) [[ e1 ]]_ None ] in
+  JFIPartialEval h0 st0 confs hn [ [] [[JFVal1 (JFVLoc res) ]]_ None] CC ->
+   (st = [] /\ ctx = [] /\ exists e1_res, e1 = JFVal1 (JFVLoc e1_res)) \/
+   (exists st' ctx' h' e1', red CC (h0, st0) = Some (h', st' ++ [ (ctx' ++ [JFCtxLet class x __ e2]) [[ e1' ]]_ None ])).
+Proof.
+  intros h0 class x e1 e2 confs hn res CC st ctx.
+  intros st0 let_eval.
+  destruct st.
+  + unfold st0 in let_eval.
+    rewrite app_nil_l in let_eval.
+    apply OnlyFrameIsValOrRedPreservesLetCtx in let_eval
+      as [(ctx_empty & exists_e1_res) | red_is_some].
+    ++ apply or_introl.
+       split; try split; try assumption.
+    ++ apply or_intror.
+       exact red_is_some.
+  + apply or_intror.
+    unfold st0 in let_eval.
+    rewrite app_split in let_eval.
+    assert (tmp := TopFrameRedPreservesLetCtx _ _ _ _ _ _ _ _ _ _ _ _ let_eval);
+    destruct tmp as (st' & ctx' & h' & e1' & red_is_some).
+    exists st', ctx', h', e1'.
+    rewrite <- app_split in red_is_some.
+    fold st0 in red_is_some.
+    exact red_is_some.
+Qed.
 
 Definition LetCtxSt ctxs class x e1 e2 :=
   [(ctxs ++ [JFCtxLet class x __ e2]) [[ e1 ]]_ None].
@@ -2046,33 +2750,38 @@ Definition LetCtxSt ctxs class x e1 e2 :=
 Definition LetCtxStInEnv ctxs class x e1 e2 env :=
   LetCtxSt ctxs class x (JFIExprSubstituteEnv env e1) (JFIExprSubstituteEnv env e2).
 
-Lemma LetInnerEvaluation : forall confs ctxs h class x e1 e2 hn res CC,
-  (JFIPartialEval h (LetCtxSt ctxs class x e1 e2) confs hn [ [] [[JFVal1 (JFVLoc res) ]]_ None] CC) ->
+Lemma LetInnerEvaluation : forall confs st ctxs h class x e1 e2 hn res CC,
+  (JFIPartialEval h (st ++ (LetCtxSt ctxs class x e1 e2)) confs hn [ [] [[JFVal1 (JFVLoc res) ]]_ None] CC) ->
    exists confs_e1 h' e1_res,
-     JFIPartialEval h (LetCtxSt ctxs class x e1 e2) confs_e1 h' (LetCtxSt [] class x (JFVal1 (JFVLoc e1_res)) e2) CC /\
-     forall conf, In conf confs_e1 -> exists conf_h ctxs' e1', conf = (conf_h, LetCtxSt (ctxs' ++ ctxs) class x e1' e2).
+     JFIPartialEval h (st ++ (LetCtxSt ctxs class x e1 e2)) confs_e1 h' (LetCtxSt [] class x (JFVal1 (JFVLoc e1_res)) e2) CC /\
+     forall conf, In conf confs_e1 -> exists conf_h st' ctxs' e1', conf = (conf_h, (st' ++ LetCtxSt ctxs' class x e1' e2)).
 Proof.
   intros confs.
   induction confs.
-  + intros ctxs h class x e1 e2 hn res CC.
+  + intros st ctxs h class x e1 e2 hn res CC.
     intros let_eval.
     simpl in let_eval.
     unfold LetCtxSt in let_eval.
     simpl in let_eval.
     destruct ctxs.
-    ++ rewrite app_nil_l in let_eval.
-       discriminate (proj2 let_eval).
-    ++ discriminate (proj2 let_eval).
-  + intros ctxs h class x e1 e2 hn res CC.
+    ++ destruct let_eval as (_ & st_eq).
+       rewrite app_nil_l in st_eq.
+       rewrite <- app_nil_l in st_eq.
+       apply app_inj_tail in st_eq.
+       discriminate (proj2 st_eq).
+    ++ destruct let_eval as (_ & st_eq).
+       rewrite <- app_nil_l in st_eq.
+       apply app_inj_tail in st_eq.
+       discriminate (proj2 st_eq).
+  + intros st ctxs h class x e1 e2 hn res CC.
     intros let_eval.
-    assert (tmp := LetCtxIsValOrRedToLetCtx h class x e1 e2(a :: confs) hn res CC ctxs).
-    assert (val_or_red_to_let_ctx := tmp let_eval); clear tmp.
-    destruct val_or_red_to_let_ctx as [(ctxs_empty & (e1_res & is_val)) | (ctx' & (h' & (e1' & red_to_let_ctx)))].
+    destruct (RedPreservesLetCtxUntilE2Evaluates h class x e1 e2(a :: confs) hn res CC st ctxs let_eval)
+        as [(st_empty & (ctxs_empty & (e1_res & is_val)))  | (st' & (ctx' & (h' & (e1' & red_to_let_ctx))))].
     ++ rewrite is_val.
        exists [], h, e1_res.
        split.
        +++ unfold JFIPartialEval.
-           rewrite ctxs_empty.
+           rewrite st_empty, ctxs_empty.
            split; try split; try trivial.
        +++ intros conf conf_in_nil.
            destruct conf_in_nil.
@@ -2081,19 +2790,17 @@ Proof.
        destruct let_eval as (h_eq_h0 & (st_eq_f & let_red)).
        rewrite st_eq_f in let_red.
 
-       replace [(ctxs ++
+       replace (st ++ [(ctxs ++
                      [JFCtxLet class x __ e2])
-                    [[ e1 ]]_ None] with f in red_to_let_ctx.
+                    [[ e1 ]]_ None]) with f in red_to_let_ctx.
        replace (red CC (h, f) ) with (Some
                    (h',
-                   [(ctx' ++
-                     ctxs ++
+                   (st' ++ [(ctx' ++
                      [JFCtxLet class x __ e2])
-                    [[e1' ]]_ None])) in let_red.
+                    [[e1' ]]_ None]))) in let_red.
        fold JFIPartialEval in let_red.
 
        unfold LetCtxStInEnv, LetCtxSt in IHconfs.
-       rewrite app_assoc in let_red.
        apply IHconfs in let_red.
 
        destruct let_red as
@@ -2106,31 +2813,27 @@ Proof.
            rewrite st_eq_f.
            replace (red CC (h, f) ) with (Some
                    (h',
-                   [(ctx' ++ ctxs ++ [JFCtxLet class x __ e2]) [[e1'
-                    ]]_ None])).
+                   (st' ++ [(ctx' ++ [JFCtxLet class x __ e2]) [[ e1' ]]_ None]))).
            fold JFIPartialEval.
-           rewrite app_assoc.
            exact eval_e1'.
        +++ intros conf conf_in_confs.
            apply in_inv in conf_in_confs.
            destruct conf_in_confs as [conf_eq_h_f | conf_in_confs].
            - destruct conf as (conf_h, conf_f).
-             exists h, [], e1.
-             rewrite app_nil_l.
+             exists h, st, ctxs, e1.
              rewrite st_eq_f.
              symmetry.
              exact conf_eq_h_f.
            - assert (exists_conf_h := confs_e1'_let_ctx conf conf_in_confs).
-             destruct (confs_e1'_let_ctx conf conf_in_confs) as (conf_h & (ctxs' & (e1'' & conf_h_st_l))).
+             destruct (confs_e1'_let_ctx conf conf_in_confs) as (conf_h & (st'' & (ctx'' & (e1'' & conf_h_st_l)))).
              unfold LetCtxSt.
-             exists conf_h, (ctxs' ++ ctx'), e1''.
+             exists conf_h, st'', ctx'', e1''.
              rewrite conf_h_st_l.
-             rewrite app_assoc.
              trivial.
 Qed.
 
 Definition E1ConfIsStrippedLetConf (e1_conf conf : Heap * FrameStack) class x e2 :=
-  fst e1_conf = fst conf /\ exists ctxs e1, snd e1_conf = [ctxs [[ e1 ]]_ None] /\ snd conf = LetCtxSt ctxs class x e1 e2.
+  fst e1_conf = fst conf /\ exists st ctxs e1, snd e1_conf = st ++ [ctxs [[ e1 ]]_ None] /\ snd conf = st ++ LetCtxSt ctxs class x e1 e2.
 
 Fixpoint E1ConfsAreStrippedLetConfs e1_confs confs class x e2:=
   match (e1_confs, confs) with
@@ -2149,16 +2852,16 @@ Proof.
   exact H0.
 Qed.
 
-Lemma ForStripedConfExistLetContext : forall e1_h e1_st h st class x e2,
-  E1ConfIsStrippedLetConf (e1_h, e1_st) (h, st) class x e2 ->
-  exists ctx e1, 
-   [(ctx ++ [JFCtxLet class x __ e2]) [[ e1 ]]_ None] = st /\
-   [ ctx [[ e1 ]]_ None] = e1_st.
+Lemma ForStripedConfExistLetContext : forall e1_h e1_st let_h let_st class x e2,
+  E1ConfIsStrippedLetConf (e1_h, e1_st) (let_h, let_st) class x e2 ->
+  exists st ctx e1, 
+   st ++ [(ctx ++ [JFCtxLet class x __ e2]) [[ e1 ]]_ None] = let_st /\
+   st ++ [ ctx [[ e1 ]]_ None] = e1_st.
 Proof.
   intros.
   unfold E1ConfIsStrippedLetConf in H.
-  destruct H as (_ & (ctx & (e1 & (e1_st_eq & st_eq)))).
-  exists ctx, e1.
+  destruct H as (_ & st & ctx & e1 & e1_st_eq & st_eq).
+  exists st, ctx, e1.
   split.
   + unfold LetCtxSt, snd in st_eq.
     symmetry.
@@ -2181,7 +2884,7 @@ Proof.
 Qed.
 
 Lemma ExistsStrippedInnerLetEvaluation : forall confs class x e2,
-  (forall conf, In conf confs -> exists conf_h ctxs' e1', conf = (conf_h, LetCtxSt (ctxs' ++ []) class x e1' e2)) ->
+  (forall conf, In conf confs -> exists conf_h st' ctxs' e1', conf = (conf_h, st' ++ LetCtxSt ctxs' class x e1' e2)) ->
   exists e1_confs, E1ConfsAreStrippedLetConfs e1_confs confs class x e2.
 Proof.
   intros confs class x e2.
@@ -2191,51 +2894,31 @@ Proof.
     simpl.
     trivial.
   + destruct (forall_conf_confs_exists_stripped_conf conf (List.in_eq conf confs))
-      as (e1_h & (ctxs' & (e1' & conf_eq))).
+      as (e1_h & st' & ctxs' & e1' & conf_eq).
     assert (e1_confs : forall conf0 : Heap * list Frame,
                In conf0 confs ->
-               exists (conf_h : Heap) (ctxs' : list JFContextNode) (e1' : JFExpr),
-                 conf0 = (conf_h, LetCtxSt (ctxs' ++ []) class x e1' e2));
+               exists (conf_h : Heap) st' (ctxs' : list JFContextNode) (e1' : JFExpr),
+                 conf0 = (conf_h, st' ++ LetCtxSt ctxs' class x e1' e2));
       [apply StrenghtenInAssumption with (h := conf);
        exact forall_conf_confs_exists_stripped_conf |].
     apply IHconfs in e1_confs as (e1_confs & e1_confs_stripped).
     unfold LetCtxSt in conf_eq.
-    exists ((e1_h, [ ctxs' [[ e1' ]]_ None])::e1_confs).
+    exists ((e1_h, st' ++ [ctxs' [[ e1' ]]_ None])::e1_confs).
     simpl.
     split.
     ++ rewrite conf_eq.
        unfold E1ConfIsStrippedLetConf, fst, snd.
        split; trivial.
-       exists ctxs', e1'.
+       exists st', ctxs', e1'.
        unfold LetCtxSt.
-       rewrite app_nil_r.
        split; trivial.
     ++ exact e1_confs_stripped.
 Qed.
 
-Lemma RedIsNoneIsFalseImpliesRedIsSome : forall CC conf p,
-  match red CC conf with
-  | Some (h, st) => p h st
-  | None => False
-  end -> exists h st, (red CC conf = Some (h, st) /\ p h st).
-Proof.
-  intros.
-  destruct (Classical_Prop.classic (exists h st, red CC conf = Some (h, st))).
-  + destruct H0 as (h & (st & red_is_some)).
-    exists h, st.
-    rewrite red_is_some in H.
-    exact (conj red_is_some H).
-  + destruct (red CC conf).
-    ++ destruct p0.
-       exists h, f.
-       split; try trivial.
-    ++ destruct H.
-Qed.
-
-Lemma StrippedRedExists : forall h ctx class x e1 e2 h' ctx' e1' CC,
-  red CC (h, [(ctx ++ [JFCtxLet class x __ e2]) [[ e1 ]]_ None]) =
-     Some (h', [(ctx' ++ [JFCtxLet class x __ e2]) [[ e1' ]]_ None]) ->
-  red CC (h, [ctx [[ e1 ]]_ None]) =  Some (h', [ctx' [[ e1' ]]_ None]).
+Lemma StrippedRedExists : forall h st ctx class x e1 e2 h' st' ctx' e1' CC,
+  red CC (h, st ++ [(ctx ++ [JFCtxLet class x __ e2]) [[ e1 ]]_ None]) =
+     Some (h', st' ++ [(ctx' ++ [JFCtxLet class x __ e2]) [[ e1' ]]_ None]) ->
+  red CC (h, st ++ [ctx [[ e1 ]]_ None]) =  Some (h', st' ++ [ctx' [[ e1' ]]_ None]).
 Proof.
 Admitted.
 
@@ -2265,43 +2948,45 @@ Proof.
   auto.
 Qed.
 
-Lemma StripConf : forall ctx class x e1 e2 e1_h e1_st let_h let_st,
-  [(ctx ++ [JFCtxLet class x __ e2]) [[e1 ]]_ None] = let_st ->
+Lemma StripConf : forall st ctx class x e1 e2 e1_h e1_st let_h let_st,
+  st ++ [(ctx ++ [JFCtxLet class x __ e2]) [[e1 ]]_ None] = let_st ->
   E1ConfIsStrippedLetConf (e1_h, e1_st) (let_h, let_st) class x e2 ->
-  [ctx [[e1 ]]_ None] = e1_st.
+  st ++ [ctx [[e1 ]]_ None] = e1_st.
 Proof.
   intros.
   unfold E1ConfIsStrippedLetConf, snd in H0.
-  destruct H0 as (_ & (ctx' & (e1' & (e1_st_eq & let_st_eq')))).
+  destruct H0 as (_ & st' & ctx' & e1' & e1_st_eq & let_st_eq').
   rewrite e1_st_eq.
   rewrite <- H in let_st_eq'.
   unfold LetCtxSt in let_st_eq'.
+  apply app_inj_tail in let_st_eq' as (st_eq_st' & let_st_eq').
   injection let_st_eq' as tmp.
   apply app_inj_tail in tmp as (ctx_eq_ctx' & _).
-  rewrite ctx_eq_ctx', H0.
+  rewrite st_eq_st', ctx_eq_ctx', H0.
   trivial.
 Qed.
 
-Lemma StrippedInnerLetEvaluationIsE1Evaluation : forall e1_confs h ctx class x e1 e2 confs hn e1_res CC,
-  JFIPartialEval h (LetCtxSt ctx class x e1 e2) confs hn (LetCtxSt [] class x (JFVal1 (JFVLoc e1_res)) e2) CC ->
+Lemma StrippedInnerLetEvaluationIsE1Evaluation : forall e1_confs h st ctx class x e1 e2 confs hn e1_res CC,
+  JFIPartialEval h (st ++ (LetCtxSt ctx class x e1 e2)) confs hn (LetCtxSt [] class x (JFVal1 (JFVLoc e1_res)) e2) CC ->
   E1ConfsAreStrippedLetConfs e1_confs confs class x e2 ->
-  JFIPartialEval h [ ctx [[ e1 ]]_ None] e1_confs hn [ [] [[JFVal1 (JFVLoc e1_res) ]]_ None] CC.
+  JFIPartialEval h (st ++ [ ctx [[ e1 ]]_ None]) e1_confs hn [ [] [[JFVal1 (JFVLoc e1_res) ]]_ None] CC.
 Proof.
   intros e1_confs.
   unfold LetCtxSt.
 
   induction e1_confs;
-    intros h ctx class x e1 e2 confs hn e1_res CC;
+    intros h st ctx class x e1 e2 confs hn e1_res CC;
     intros inner_eval confs_stripped;
     destruct confs; try destruct confs_stripped.
   + unfold JFIPartialEval in inner_eval.
     destruct inner_eval as (h_eq_hn & inner_eval).
+    rewrite <- app_nil_l in inner_eval.
+    apply app_inj_tail in inner_eval as (st_empty & inner_eval).
     injection inner_eval.
     intros e1_is_val ctx_is_nil.
     rewrite <- app_nil_l in ctx_is_nil.
     apply app_inv_tail in ctx_is_nil.
-    rewrite ctx_is_nil.
-    rewrite e1_is_val.
+    rewrite ctx_is_nil, e1_is_val, st_empty.
     unfold JFIPartialEval.
     auto.
   + destruct e1_confs; destruct confs; try destruct H0.
@@ -2316,7 +3001,7 @@ Proof.
        +++ apply RedIsNoneIsFalseImpliesRedIsSome in let_red
              as (h0' & (st' & (red_is_some & (h'_eq & st'_eq)))).
            rewrite h'_eq, st'_eq in *.
-           set (strip_red := StrippedRedExists h ctx class x e1 e2 hn []).
+           assert (strip_red := StrippedRedExists h st ctx class x e1 e2 hn [] []).
            rewrite app_nil_l in strip_red.
            apply strip_red in red_is_some.
            apply rewrite_red.
@@ -2334,25 +3019,25 @@ Proof.
        +++ apply StripConf with (class := class) (x := x) (e2 := e2) (e1_h := e1_h)
                 (let_h := let_h) (let_st := let_st); try assumption.
        +++ apply RedIsNoneIsFalseImpliesRedIsSome in let_red
-             as (h0' & (st' & (red_is_some & inner_eval))).
+             as (h0' & (st0' & (red_is_some & inner_eval))).
 
            assert (tmp := inner_eval).
            unfold confs' in tmp.
            unfold JFIPartialEval in tmp.
            destruct p1.
-           destruct tmp as (h0'_eq_h0 & (st'_eq_f & _)).
-           rewrite h0'_eq_h0, st'_eq_f in *.
-           clear h0'_eq_h0 st'_eq_f h0'.
+           destruct tmp as (h0'_eq_h0 & (st0'_eq_f & _)).
+           rewrite h0'_eq_h0, st0'_eq_f in *.
+           clear h0'_eq_h0 st0'_eq_f h0'.
 
            assert (p0_stripped := H0).
            apply ForStripedConfExistLetContext in H0
-              as (ctx' & (e1' & (f_eq & p0_eq))).
+              as (st' & ctx' & e1' & f_eq & p0_eq).
            rewrite <- f_eq in red_is_some.
 
-           assert (strip_red := StrippedRedExists h ctx class x e1 e2 h0 ctx').
+           assert (strip_red := StrippedRedExists h st ctx class x e1 e2 h0 st' ctx').
            apply strip_red in red_is_some.
            apply rewrite_red1 with
-                  (h' := h0) (st' := [ctx' [[e1' ]]_ None]); try assumption.
+                  (h' := h0) (st' := st' ++ [ctx' [[e1' ]]_ None]); try assumption.
            apply IHe1_confs with (class := class) (x := x) (e2 := e2) (confs := confs').
            - rewrite f_eq.
              apply inner_eval.
@@ -2363,7 +3048,7 @@ Qed.
 
 Lemma LetE1Evaluation : forall h class x e1 e1_res e2 confs hn CC,
   (JFIPartialEval h (LetCtxSt [] class x e1 e2) confs hn (LetCtxSt [] class x (JFVal1 (JFVLoc e1_res)) e2) CC /\
-    forall conf, In conf confs -> exists conf_h ctxs' e1', conf = (conf_h, LetCtxSt (ctxs' ++ []) class x e1' e2)) ->
+    forall conf, In conf confs -> exists conf_h st' ctxs' e1', conf = (conf_h, st' ++ LetCtxSt ctxs' class x e1' e2)) ->
    exists confs_e1,
      JFIPartialEval h [ [] [[ e1 ]]_ None] confs_e1 hn
         [ [] [[ JFVal1 (JFVLoc e1_res) ]]_ None] CC.
@@ -2372,7 +3057,7 @@ Proof.
   intros (inner_eval & confs_in_let_ctx).
   apply ExistsStrippedInnerLetEvaluation in confs_in_let_ctx as (e1_confs & e1_confs_are_stripped_confs).
   exists e1_confs.
-  apply StrippedInnerLetEvaluationIsE1Evaluation with (class := class) (x := x) (e2 := e2) (confs := confs); assumption.
+  apply StrippedInnerLetEvaluationIsE1Evaluation with (st := []) (class := class) (x := x) (e2 := e2) (confs := confs); assumption.
 Qed.
 
 Lemma LetGoEvaluationStep : forall h class x env e1_res e2 confs_let_e2 hn res CC,
@@ -2417,9 +3102,10 @@ Proof.
     fold JFIPartialEval in let_eval.
     unfold red in let_eval.
     assert (tmp := let_eval).
-    apply (LetInnerEvaluation confs []) in tmp as (confs_let_e1 & (h' & (e1_res & e1_eval))).
+    apply (LetInnerEvaluation confs [] []) in tmp as (confs_let_e1 & (h' & (e1_res & e1_eval))).
     assert (e1_let_eval := e1_eval).
     destruct e1_let_eval as (e1_let_eval & _).
+    rewrite app_nil_l in e1_eval.
     apply LetE1Evaluation in e1_eval as (confs_e1 & e1_eval).
     unfold LetCtxSt in e1_let_eval.
     rewrite app_nil_l in e1_let_eval.
